eve/Src/framework/eiffel2boogie/iv/iv_goto.e
@@ -13,9 +13,15 @@ inherit
 	IV_STATEMENT
 
 create
-	make
+	make, make_empty
 
 feature {NONE} -- Initialization
+
+	make_empty
+			-- Initialize goto statement without targets.
+		do
+			create blocks.make
+		end
 
 	make (a_block: IV_BLOCK)
 			-- Initialize goto statement with target `a_block'.
